@base <https://cube.link/>.

@prefix rdf: <http://www.w3.org/1999/02/22-rdf-syntax-ns#>.
@prefix rdfs: <http://www.w3.org/2000/01/rdf-schema#>.


# Core Schema

<>
  rdfs:label "Cube Schema".

<Constraint> a rdfs:Class;
  rdfs:label "Constraint";
  rdfs:comment "Specifies constraints that need to be met on the Cube. Used for metadata and validation.".

<Cube> a rdfs:Class;
  rdfs:label "Cube";
  rdfs:comment "Represents the entry point for a collection of observations, conforming to some common dimensional structure.".

<Observation> a rdfs:Class;
  rdfs:label "Observation";
  rdfs:comment "A single observation in the cube, may have one or more associated dimensions.".

<ObservationSet> a rdfs:Class;
  rdfs:label "Observation Set";
  rdfs:comment "A set of observations.".

<observation> a rdf:Property;
  rdfs:range <Observation>;
  rdfs:domain <ObservationSet>;
  rdfs:label "observation";
  rdfs:comment "Connects a set of observations with a single observation.".

<observationConstraint> a rdf:Property;
  rdfs:range <Constraint>;
  rdfs:domain <Cube>;
  rdfs:label "observation constraint";
  rdfs:comment "Connects a cube with a constraint for metadata and validation.".

<observationSet> a rdf:Property;
  rdfs:range <ObservationSet>;
  rdfs:domain <Cube>;
  rdfs:label "observation set";
  rdfs:comment "Connects a cube with a set of observations.".

<observedBy> a rdf:Property;
  rdfs:domain <Observation>;
  rdfs:range rdfs:Resource;
  rdfs:label "observed by";
  rdfs:comment "Connects an observation with the agent that created the observation. The agent can be a person, organisation, device or software. A description of the method to gather the data could be attached to the agent.".

<Undefined> a rdfs:Datatype;
  rdfs:label "Undefined observation.";
  rdfs:comment "An observation which is not defined.".

<KeyDimension> a rdfs:Class;
  rdfs:label "Key Dimension";
  rdfs:comment "The KeyDimension tags one or multiple dimensions which are together uniquely identifying an observation. You can think of them as the Key in a relational database.";
  .

<MeasureDimension> a rdfs:Class;
  rdfs:label "Measure Dimension";
  rdfs:comment "The MeasureDimension tags at least one dimension, but potentially multiple, which is the actual measurement, or statistical count attached to an observation.".

